dev/lf/paths/tight/Weakening.v
@@ -7,29 +7,27 @@ Require Import Definitions.
 (* ###################################################################### *)
 (** ** Weakening *)
 
-Definition foo G x T d D := G ; x ~ T ⊢ d ∈ D.
-
 Lemma weaken_rules:
-  (forall G t T, G ⊢ t ∈ T -> forall G1 G2 G3,
+  (forall G t T, G |- t :: T -> forall G1 G2 G3,
     G = G1 & G3 ->
     ok (G1 & G2 & G3) ->
-    (G1 & G2 & G3) ⊢ t ∈ T) /\
-  (forall G x T d D, G ;; x ~ T ⊢ d ∈ D -> forall G1 G2 G3,
+    G1 & G2 & G3 |- t :: T) /\
+  (forall G x T d D, G && x ~ T |- d :: D -> forall G1 G2 G3,
     G = G1 & G3 ->
     ok (G1 & G2 & G3 & x ~ T) ->
-    (G1 & G2 & G3) ;; x ~ T ⊢ d ∈ D) /\
-  (forall G x U ds T, G; x ~ U ⊢ ds ∈ T -> forall G1 G2 G3,
+    (G1 & G2 & G3) && x ~ T |- d :: D) /\
+  (forall G x U ds T, G && x ~ U |- ds ::: T -> forall G1 G2 G3,
     G = G1 & G3 ->
     ok (G1 & G2 & G3 & x ~ U) ->
-    (G1 & G2 & G3); x ~ U ⊢ ds ∈ T) /\
+    G1 & G2 & G3 && x ~ U |- ds ::: T) /\
   (forall G p, norm G p -> forall G1 G2 G3,
     G = G1 & G3 ->
     ok (G1 & G2 & G3) ->
     norm (G1 & G2 & G3) p) /\
-  (forall m1 G T U, G ⊢s T <: U -> forall G1 G2 G3,
+  (forall G T U, G |- T <: U -> forall G1 G2 G3,
     G = G1 & G3 ->
     ok (G1 & G2 & G3) ->
-    (G1 & G2 & G3) ⊢s T <: U).
+    G1 & G2 & G3 |- T <: U).
 Proof.
   apply rules_mutind; eauto 4; intros; subst.
   + eapply ty_var. eapply binds_weaken; eauto.
@@ -64,10 +62,10 @@ Proof.
     apply* H0.
 Qed.
 
-Lemma weaken_ty_trm:  forall m1 G1 G2 t T,
-    ty_trm m1 G1 t T ->
+Lemma weaken_ty_trm:  forall G1 G2 t T,
+    G1 |- t :: T ->
     ok (G1 & G2) ->
-    ty_trm m1 (G1 & G2) t T.
+    G1 & G2 |- t :: T.
 Proof.
   intros.
     assert (G1 & G2 = G1 & G2 & empty) as EqG. {
@@ -78,10 +76,10 @@ Proof.
   rewrite <- EqG. assumption.
 Qed.
 
-Lemma weaken_subtyp: forall m1 G1 G2 S U,
-  subtyp m1 G1 S U ->
+Lemma weaken_subtyp: forall G1 G2 S U,
+  G1 |- S <: U ->
   ok (G1 & G2) ->
-  subtyp m1 (G1 & G2) S U.
+  G1 & G2 |- S <: U.
 Proof.
   intros.
     assert (G1 & G2 = G1 & G2 & empty) as EqG. {
